fix lemmas up to line 270

Lean4bits/lemmas.lean
@@ -1,4 +1,4 @@
-import Mathlib.Data.Fintype.Basic
+import Mathlib.Data.Fintype.Card
 import Lean4bits.defs
 
 open Sum
@@ -6,290 +6,283 @@ open Sum
 variable {α β α' β' : Type} {γ : β → Type}
 
 def propagateAux (init_carry : α → Bool)
-  (next_bit : ∀ (carry : α → Bool) (bits : β → Bool),
-    (α → Bool) × Bool)
-  (x : β → ℕ → Bool) : ℕ → (α → Bool) × Bool
-| 0 := next_bit init_carry (λ i, x i 0)
-| (n+1) :=
-next_bit (propagateAux n).1 (λ i, x i (n+1))
+    (next_bit : ∀ (_carry : α → Bool) (_bits : β → Bool),
+      (α → Bool) × Bool)
+    (x : β → ℕ → Bool) : ℕ → (α → Bool) × Bool
+  | 0 => next_bit init_carry (fun i => x i 0)
+  | n+1 => next_bit (propagateAux init_carry next_bit x n).1 (fun i => x i (n+1))
 
 def propagate (init_carry : α → Bool)
-  (next_bit : ∀ (carry : α → Bool) (bits : β → Bool),
-    (α → Bool) × Bool)
-  (x : β → ℕ → Bool) (i : ℕ) : Bool :=
-(propagateAux init_carry next_bit x i).2
+    (next_bit : ∀ (_carry : α → Bool) (_bits : β → Bool),
+      (α → Bool) × Bool)
+    (x : β → ℕ → Bool) (i : ℕ) : Bool :=
+  (propagateAux init_carry next_bit x i).2
 
-@[simp] def propagate_carry (init_carry : α → Bool)
-  (next_bit : ∀ (carry : α → Bool) (bits : β → Bool),
-    (α → Bool))
-  (x : β → ℕ → Bool) : ℕ → (α → Bool)
-| 0 := next_bit init_carry (λ i, x i 0)
-| (n+1) := next_bit (propagate_carry n) (λ i, x i (n+1))
+@[simp] def propagateCarry (init_carry : α → Bool)
+    (next_bit : ∀ (_carry : α → Bool) (_bits : β → Bool),
+      (α → Bool))
+    (x : β → ℕ → Bool) : ℕ → (α → Bool)
+  | 0 => next_bit init_carry (fun i => x i 0)
+  | n+1 => next_bit (propagateCarry init_carry next_bit x n) (fun i => x i (n+1))
 
-@[simp] def propagate_carry2 (init_carry : α → Bool)
-  (next_bit : ∀ (carry : α → Bool) (bits : β → Bool),
-    (α → Bool))
-  (x : β → ℕ → Bool) : ℕ → (α → Bool)
-| 0 := init_carry
-| (n+1) := next_bit (propagate_carry2 n) (λ i, x i n)
+@[simp] def propagateCarry2 (init_carry : α → Bool)
+    (next_bit : ∀ (_carry : α → Bool) (_bits : β → Bool),
+      (α → Bool))
+    (x : β → ℕ → Bool) : ℕ → (α → Bool)
+  | 0 => init_carry
+  | n+1 => next_bit (propagateCarry2 init_carry next_bit x n) (fun i => x i n)
 
-lemma propagate_carry2_succ (init_carry : α → Bool)
-  (next_bit : ∀ (carry : α → Bool) (bits : β → Bool),
-    (α → Bool))
-  (x : β → ℕ → Bool) (n : ℕ) :
-  propagate_carry2 init_carry next_bit x (n+1) =
-  propagate_carry init_carry next_bit x n :=
-by induction n; simp *
+lemma propagateCarry2_succ (init_carry : α → Bool)
+    (next_bit : ∀ (_carry : α → Bool) (_bits : β → Bool),
+      (α → Bool))
+    (x : β → ℕ → Bool) : ∀ (n : ℕ),
+    propagateCarry2 init_carry next_bit x (n+1) =
+    propagateCarry init_carry next_bit x n
+  | 0 => rfl
+  | n+1 => by rw [propagateCarry2, propagateCarry2_succ _ _ _ n, propagateCarry]
 
 @[simp] lemma propagateAux_fst_eq_carry (init_carry : α → Bool)
-  (next_bit : ∀ (carry : α → Bool) (bits : β → Bool),
-    (α → Bool) × Bool)
-  (x : β → ℕ → Bool) : ∀ n : ℕ,
-  (propagateAux init_carry next_bit x n).1 =
-  propagate_carry init_carry (λ c b, (next_bit c b).1) x n
-| 0 := rfl
-| (n+1) := by rw [propagateAux, propagate_carry, propagateAux_fst_eq_carry]
+    (next_bit : ∀ (_carry : α → Bool) (_bits : β → Bool),
+      (α → Bool) × Bool)
+    (x : β → ℕ → Bool) : ∀ n : ℕ,
+    (propagateAux init_carry next_bit x n).1 =
+    propagateCarry init_carry (fun c b => (next_bit c b).1) x n
+  | 0 => rfl
+  | n+1 => by rw [propagateAux, propagateCarry, propagateAux_fst_eq_carry _ _ _ n]
 
 @[simp] lemma propagate_zero (init_carry : α → Bool)
-  (next_bit : ∀ (carry : α → Bool) (bits : β → Bool),
-  (α → Bool) × Bool)
-  (x : β → ℕ → Bool) :
-  propagate init_carry next_bit x 0 = (next_bit init_carry (λ i, x i 0)).2 :=
-rfl
+    (next_bit : ∀ (_carry : α → Bool) (_bits : β → Bool),
+    (α → Bool) × Bool)
+    (x : β → ℕ → Bool) :
+    propagate init_carry next_bit x 0 = (next_bit init_carry (fun i => x i 0)).2 :=
+  rfl
 
 lemma propagate_succ (init_carry : α → Bool)
-  (next_bit : ∀ (carry : α → Bool) (bits : β → Bool),
-    (α → Bool) × Bool)
-  (x : β → ℕ → Bool) (i : ℕ) :
-  propagate init_carry next_bit x (i+1) = (next_bit
-    (propagate_carry init_carry (λ c b, (next_bit c b).1) x i)
-    (λ j, x j (i+1))).2 :=
-by rw [← propagateAux_fst_eq_carry]; refl
+    (next_bit : ∀ (_carry : α → Bool) (_bits : β → Bool),
+      (α → Bool) × Bool)
+    (x : β → ℕ → Bool) (i : ℕ) :
+    propagate init_carry next_bit x (i+1) = (next_bit
+      (propagateCarry init_carry (fun c b => (next_bit c b).1) x i)
+      (λ j => x j (i+1))).2 :=
+  by rw [← propagateAux_fst_eq_carry]; rfl
 
 lemma propagate_succ2 (init_carry : α → Bool)
-  (next_bit : ∀ (carry : α → Bool) (bits : β → Bool),
-    (α → Bool) × Bool)
-  (x : β → ℕ → Bool) (i : ℕ) :
-  propagate init_carry next_bit x (i+1) = (next_bit
-    (propagate_carry2 init_carry (λ c b, (next_bit c b).1) x (i+1))
-    (λ j, x j (i+1))).2 :=
-by rw [propagate_carry2_succ, ← propagateAux_fst_eq_carry]; refl
+    (next_bit : ∀ (_carry : α → Bool) (_bits : β → Bool),
+      (α → Bool) × Bool)
+    (x : β → ℕ → Bool) (i : ℕ) :
+    propagate init_carry next_bit x (i+1) = (next_bit
+      (propagateCarry2 init_carry (λ c b => (next_bit c b).1) x (i+1))
+      (λ j => x j (i+1))).2 :=
+  by rw [propagateCarry2_succ, ← propagateAux_fst_eq_carry]; rfl
 
-lemma propagate_carry_propagate {δ : β → Type*} {β' : Type}
-    (f : ∀ a, δ a → β') : ∀ (n : ℕ) (init_carry : α → Bool)
-  (next_bit : ∀ (carry : α → Bool) (bits : β → Bool),
-    (α → Bool))
-  (init_carry_x : ∀ a, γ a → Bool)
-  (next_bit_x : ∀ a (carry : γ a → Bool) (bits : δ a → Bool),
-    (γ a → Bool) × Bool)
-  (x : β' → ℕ → Bool),
-  propagate_carry init_carry next_bit (λ a, propagate (init_carry_x a)
-    (next_bit_x a) (λ d, x (f a d))) n =
-  propagate_carry
-    (λ a : α ⊕ (Σ a, γ a), sum.elim init_carry (λ b : Σ a, γ a,
-      init_carry_x b.1 b.2) a)
-    (λ (carry : (α ⊕ (Σ a, γ a)) → Bool) (bits : β' → Bool),
-  -- first compute (propagate (init_carry_x a) (next_bit_x a) (x a) n)
-      let f : ∀ (a : β), (γ a → Bool) × Bool := λ a, next_bit_x a (λ d,
-        carry (inr ⟨a, d⟩)) (λ d, bits (f a d)) in
-      let g : (α → Bool) := (next_bit (carry ∘ inl) (λ a, (f a).2)) in
-      sum.elim g (λ x, (f x.1).1 x.2)
-    )
-    x n ∘ inl
-| 0 init_carry next_bit init_carry_x next_bit_x x := rfl
-| (n+1) init_carry next_bit init_carry_x next_bit_x x := begin
-  have := propagate_carry_propagate n,
-  clearAux_decl,
-  simp only [propagate_carry, propagate_succ, elim_inl] at *,
-  conv_lhs { simp only [this] },
-  clear this,
-  ext,
-  congr,
-  ext,
-  congr,
-  induction n with n ih,
-  { simp },
-  { simp [ih] }
-end
+lemma propagateCarry_propagate {δ : β → Type} {β' : Type}
+      (f : ∀ a, δ a → β') : ∀ (n : ℕ) (init_carry : α → Bool)
+    (next_bit : ∀ (_carry : α → Bool) (_bits : β → Bool),
+      (α → Bool))
+    (init_carry_x : ∀ a, γ a → Bool)
+    (next_bit_x : ∀ a (_carry : γ a → Bool) (_bits : δ a → Bool),
+      (γ a → Bool) × Bool)
+    (x : β' → ℕ → Bool),
+    propagateCarry init_carry next_bit (λ a => propagate (init_carry_x a)
+      (next_bit_x a) (λ d => x (f a d))) n =
+    propagateCarry
+      (λ a : α ⊕ (Σ a, γ a) => Sum.elim init_carry (λ b : Σ a, γ a =>
+        init_carry_x b.1 b.2) a)
+      (λ (carry : (α ⊕ (Σ a, γ a)) → Bool) (bits : β' → Bool) =>
+    -- first compute (propagate (init_carry_x a) (next_bit_x a) (x a) n)
+        let f : ∀ (a : β), (γ a → Bool) × Bool := λ a => next_bit_x a
+          (λ d => carry (inr ⟨a, d⟩)) (λ d => bits (f a d))
+        let g : (α → Bool) := (next_bit (carry ∘ inl) (λ a => (f a).2))
+        Sum.elim g (λ x => (f x.1).1 x.2))
+      x n ∘ inl
+  | 0, init_carry, next_bit, init_carry_x, next_bit_x, x => rfl
+  | n+1, init_carry, next_bit, init_carry_x, next_bit_x, x => by
+    have := propagateCarry_propagate f n
+    simp only [propagateCarry, propagate_succ, elim_inl, Nat.add] at *
+    conv_lhs => simp only [this]
+    clear this
+    dsimp
+    congr
+    ext a
+    dsimp
+    congr
+    ext b
+    dsimp [propagateCarry, propagate_succ, elim_inl, Nat.add]
+    congr
+    dsimp
+    induction' n with n ih
+    . simp
+    . simp [ih]
 
-lemma propagate_propagate {δ : β → Type*} {β' : Type}
-    (f : ∀ a, δ a → β') : ∀ (n : ℕ) (init_carry : α → Bool)
-  (next_bit : ∀ (carry : α → Bool) (bits : β → Bool),
-    (α → Bool) × Bool)
-  (init_carry_x : ∀ a, γ a → Bool)
-  (next_bit_x : ∀ a (carry : γ a → Bool) (bits : δ a → Bool),
-    (γ a → Bool) × Bool)
-  (x : β' → ℕ → Bool),
-  propagate init_carry next_bit (λ a, propagate (init_carry_x a)
-    (next_bit_x a) (λ d, x (f a d))) n =
-  propagate
-    (λ a : α ⊕ (Σ a, γ a), sum.elim init_carry (λ b : Σ a, γ a,
-      init_carry_x b.1 b.2) a)
-    (λ (carry : (α ⊕ (Σ a, γ a)) → Bool) (bits : β' → Bool),
-      -- first compute (propagate (init_carry_x a) (next_bit_x a) (x a) n)
-      let f : ∀ (a : β), (γ a → Bool) × Bool := λ a, next_bit_x a (λ d,
-        carry (inr ⟨a, d⟩)) (λ d, bits (f a d)) in
-      let g : (α → Bool) × Bool := (next_bit (carry ∘ inl) (λ a, (f a).2)) in
-      (sum.elim g.1 (λ x, (f x.1).1 x.2), g.2)
-    )
-  x n
-| 0 init_carry next_bit init_carry_x next_bit_x x := rfl
-| (n+1) init_carry next_bit init_carry_x next_bit_x x := begin
-  simp only [propagate_succ],
-  clearAux_decl,
-  rw [propagate_carry_propagate],
-  congr,
-  ext,
-  congr,
-  induction n with n ih,
-  { simp },
-  { simp [ih] }
-end
+lemma propagate_propagate {δ : β → Type} {β' : Type}
+      (f : ∀ a, δ a → β') : ∀ (n : ℕ) (init_carry : α → Bool)
+    (next_bit : ∀ (_carry : α → Bool) (_bits : β → Bool),
+      (α → Bool) × Bool)
+    (init_carry_x : ∀ a, γ a → Bool)
+    (next_bit_x : ∀ a (_carry : γ a → Bool) (_bits : δ a → Bool),
+      (γ a → Bool) × Bool)
+    (x : β' → ℕ → Bool),
+    propagate init_carry next_bit (λ a => propagate (init_carry_x a)
+      (next_bit_x a) (λ d => x (f a d))) n =
+    propagate
+      (λ a : α ⊕ (Σ a, γ a) => Sum.elim init_carry (λ b : Σ a, γ a =>
+        init_carry_x b.1 b.2) a)
+      (λ (carry : (α ⊕ (Σ a, γ a)) → Bool) (bits : β' → Bool) =>
+        -- first compute (propagate (init_carry_x a) (next_bit_x a) (x a) n)
+        let f : ∀ (a : β), (γ a → Bool) × Bool := λ a => next_bit_x a (λ d =>
+          carry (inr ⟨a, d⟩)) (λ d => bits (f a d))
+        let g : (α → Bool) × Bool := (next_bit (carry ∘ inl) (λ a => (f a).2))
+        (Sum.elim g.1 (λ x => (f x.1).1 x.2), g.2)
+      )
+    x n
+  | 0, init_carry, next_bit, init_carry_x, next_bit_x, x => rfl
+  | n+1, init_carry, next_bit, init_carry_x, next_bit_x, x => by
+    simp only [propagate_succ]
+    rw [propagateCarry_propagate]
+    congr
+    ext
+    congr
+    induction' n with n ih
+    . simp
+    . simp [ih]
 
-lemma propagate_carry_change_vars {β' : Type}
-  (init_carry : α → Bool)
-  (next_bit : ∀ (carry : α → Bool) (bits : β → Bool),
-    (α → Bool))
-  (x : β' → ℕ → Bool) (i : ℕ)
-  (change_vars : β → β') :
-  propagate_carry init_carry next_bit (λ b, x (change_vars b)) i =
-  propagate_carry init_carry (λ (carry : α → Bool) (bits : β' → Bool),
-    next_bit carry (λ b, bits (change_vars b))) x i :=
-begin
-  induction i,
-  { simp },
-  { simp * }
-end
+lemma propagateCarry_changeVars {β' : Type}
+    (init_carry : α → Bool)
+    (next_bit : ∀ (_carry : α → Bool) (_bits : β → Bool),
+      (α → Bool))
+    (x : β' → ℕ → Bool) (i : ℕ)
+    (changeVars : β → β') :
+    propagateCarry init_carry next_bit (λ b => x (changeVars b)) i =
+    propagateCarry init_carry (λ (carry : α → Bool) (bits : β' → Bool) =>
+      next_bit carry (λ b => bits (changeVars b))) x i := by
+  induction i
+  . simp
+  . simp [*]
 
-lemma propagate_change_vars {β' : Type}
-  (init_carry : α → Bool)
-  (next_bit : ∀ (carry : α → Bool) (bits : β → Bool),
-    (α → Bool) × Bool)
-  (x : β' → ℕ → Bool) (i : ℕ)
-  (change_vars : β → β') :
-  propagate init_carry next_bit (λ b, x (change_vars b)) i =
-  propagate init_carry (λ (carry : α → Bool) (bits : β' → Bool),
-    next_bit carry (λ b, bits (change_vars b))) x i :=
-begin
-  induction i with i ih,
-  { refl },
-  { simp only [propagate_succ, propagate_carry_change_vars, ih] }
-end
+lemma propagate_changeVars {β' : Type}
+    (init_carry : α → Bool)
+    (next_bit : ∀ (_carry : α → Bool) (_bits : β → Bool),
+      (α → Bool) × Bool)
+    (x : β' → ℕ → Bool) (i : ℕ)
+    (changeVars : β → β') :
+    propagate init_carry next_bit (λ b => x (changeVars b)) i =
+    propagate init_carry (λ (carry : α → Bool) (bits : β' → Bool) =>
+      next_bit carry (λ b => bits (changeVars b))) x i := by
+  induction' i with i ih
+  . rfl
+  . simp only [propagate_succ, propagateCarry_changeVars, ih]
 
-open term
+open Term
 
-@[simp] def arity : term → ℕ
-| (var n) := n+1
-| zero := 0
-| one := 0
-| neg_one := 0
-| (and t₁ t₂) := max (arity t₁) (arity t₂)
-| (or t₁ t₂) := max (arity t₁) (arity t₂)
-| (xor t₁ t₂) := max (arity t₁) (arity t₂)
-| (not t) := arity t
-| (ls t) := arity t
-| (add t₁ t₂) := max (arity t₁) (arity t₂)
-| (sub t₁ t₂) := max (arity t₁) (arity t₂)
-| (neg t) := arity t
-| (incr t) := arity t
-| (decr t) := arity t
+@[simp] def arity : Term → ℕ
+| (var n) => n+1
+| zero => 0
+| one => 0
+| neg_one => 0
+| Term.and t₁ t₂ => max (arity t₁) (arity t₂)
+| Term.or t₁ t₂ => max (arity t₁) (arity t₂)
+| Term.xor t₁ t₂ => max (arity t₁) (arity t₂)
+| Term.not t => arity t
+| ls t => arity t
+| add t₁ t₂ => max (arity t₁) (arity t₂)
+| sub t₁ t₂ => max (arity t₁) (arity t₂)
+| neg t => arity t
+| incr t => arity t
+| decr t => arity t
 
-@[simp] def term.eval_fin : ∀ (t : term) (vars : fin (arity t) → ℕ → Bool), ℕ → Bool
-| (var n) vars := vars (fin.last n)
-| zero vars := zero_seq
-| one vars := one_seq
-| neg_one vars := neg_one_seq
-| (and t₁ t₂) vars :=
-  and_seq (term.eval_fin t₁
-    (λ i, vars (fin.cast_le (by simp [arity]) i)))
-  (term.eval_fin t₂
-    (λ i, vars (fin.cast_le (by simp [arity]) i)))
-| (or t₁ t₂) vars :=
-  or_seq (term.eval_fin t₁
-    (λ i, vars (fin.cast_le (by simp [arity]) i)))
-  (term.eval_fin t₂
-    (λ i, vars (fin.cast_le (by simp [arity]) i)))
-| (xor t₁ t₂) vars :=
-  xor_seq (term.eval_fin t₁
-    (λ i, vars (fin.cast_le (by simp [arity]) i)))
-  (term.eval_fin t₂
-    (λ i, vars (fin.cast_le (by simp [arity]) i)))
-| (not t) vars := not_seq (term.eval_fin t vars)
-| (ls t) vars := ls_seq (term.eval_fin t vars)
-| (add t₁ t₂) vars :=
-  add_seq (term.eval_fin t₁
-    (λ i, vars (fin.cast_le (by simp [arity]) i)))
-  (term.eval_fin t₂
-    (λ i, vars (fin.cast_le (by simp [arity]) i)))
-| (sub t₁ t₂) vars :=
-  sub_seq (term.eval_fin t₁
-    (λ i, vars (fin.cast_le (by simp [arity]) i)))
-  (term.eval_fin t₂
-    (λ i, vars (fin.cast_le (by simp [arity]) i)))
-| (neg t) vars := neg_seq (term.eval_fin t vars)
-| (incr t) vars := incr_seq (term.eval_fin t vars)
-| (decr t) vars := decr_seq (term.eval_fin t vars)
+@[simp] def Term.evalFin : ∀ (t : Term) (_vars : Fin (arity t) → ℕ → Bool), ℕ → Bool
+| var n, vars => vars (Fin.last n)
+| zero, _vars => zeroSeq
+| one, _vars => oneSeq
+| neg_one, _vars => negOneSeq
+| Term.and t₁ t₂, vars =>
+  andSeq (Term.evalFin t₁
+    (fun i => vars (Fin.castLe (by simp [arity]) i)))
+  (Term.evalFin t₂
+    (fun i => vars (Fin.castLe (by simp [arity]) i)))
+| Term.or t₁ t₂, vars =>
+  orSeq (Term.evalFin t₁
+    (fun i => vars (Fin.castLe (by simp [arity]) i)))
+  (Term.evalFin t₂
+    (fun i => vars (Fin.castLe (by simp [arity]) i)))
+| Term.xor t₁ t₂, vars =>
+  xorSeq (Term.evalFin t₁
+    (fun i => vars (Fin.castLe (by simp [arity]) i)))
+  (Term.evalFin t₂
+    (fun i => vars (Fin.castLe (by simp [arity]) i)))
+| not t, vars => notSeq (Term.evalFin t vars)
+| ls t, vars => lsSeq (Term.evalFin t vars)
+| add t₁ t₂, vars =>
+  addSeq (Term.evalFin t₁
+    (fun i => vars (Fin.castLe (by simp [arity]) i)))
+  (Term.evalFin t₂
+    (fun i => vars (Fin.castLe (by simp [arity]) i)))
+| sub t₁ t₂, vars =>
+  subSeq (Term.evalFin t₁
+    (fun i => vars (Fin.castLe (by simp [arity]) i)))
+  (Term.evalFin t₂
+    (fun i => vars (Fin.castLe (by simp [arity]) i)))
+| neg t, vars => negSeq (Term.evalFin t vars)
+| incr t, vars => incrSeq (Term.evalFin t vars)
+| decr t, vars => decrSeq (Term.evalFin t vars)
 
-lemma eval_fin_eq_eval (t : term) (vars : ℕ → ℕ → Bool) :
-  term.eval_fin t (λ i, vars i) = term.eval t vars :=
-begin
-  induction t;
-  dsimp [term.eval_fin, term.eval, arity] at *; simp *
-end
+lemma evalFin_eq_eval (t : Term) (vars : ℕ → ℕ → Bool) :
+    Term.evalFin t (fun i => vars i) = Term.eval t vars := by
+  induction t <;>
+  dsimp [Term.evalFin, Term.eval, arity] at * <;> simp [*]
+
 
 lemma id_eq_propagate (x : ℕ → Bool) :
-  x = propagate empty.elim (λ _ (y : unit → Bool), (empty.elim, y ())) (λ _, x) :=
-by ext n; cases n; refl
+    x = propagate Empty.elim (λ _ (y : Unit → Bool) => (Empty.elim, y ())) (λ _ => x) := by
+  ext n; cases n <;> rfl
 
 lemma zero_eq_propagate :
-  zero_seq = propagate empty.elim (λ (_ _ : empty → Bool), (empty.elim, ff)) empty.elim :=
-by ext n; cases n; refl
+    zeroSeq = propagate Empty.elim (λ (_ _ : Empty → Bool) => (Empty.elim, false)) Empty.elim := by
+  ext n; cases n <;> rfl
 
 lemma one_eq_propagate :
-  one_seq = propagate (λ _ : unit, tt) (λ f (_ : empty → Bool), (λ _, ff, f ())) empty.elim :=
-begin
-  ext n,
-  cases n with n,
-  { refl },
-  { cases n,
-    { simp [one_seq, propagate_succ] },
-    { simp [one_seq, propagate_succ] } }
-end
+    oneSeq = propagate (λ _ : Unit => true)
+      (λ f (_ : Empty → Bool) => (λ _ => false, f ())) Empty.elim := by
+  ext n
+  match n with
+  | 0 => rfl
+  | 1 => rfl
+  | n+2 => simp [oneSeq, propagate_succ]
 
 lemma and_eq_propagate (x y : ℕ → Bool) :
-  and_seq x y = propagate empty.elim
-    (λ _ (y : Bool → Bool), (empty.elim, y tt && y ff)) (λ b, cond b x y) :=
-by ext n; cases n; simp [propagate, propagateAux, and_seq]
+    andSeq x y = propagate Empty.elim
+      (λ _ (y : Bool → Bool) => (Empty.elim, y true && y false)) (λ b => cond b x y) := by
+  ext n; cases n <;> simp [propagate, propagateAux, andSeq]
 
 lemma or_eq_propagate (x y : ℕ → Bool) :
-  or_seq x y = propagate empty.elim
-    (λ _ (y : Bool → Bool), (empty.elim, y tt || y ff)) (λ b, cond b x y) :=
-by ext n; cases n; simp [propagate, propagateAux, or_seq]
+    orSeq x y = propagate Empty.elim
+      (λ _ (y : Bool → Bool) => (Empty.elim, y true || y false)) (λ b => cond b x y) := by
+  ext n; cases n <;> simp [propagate, propagateAux, orSeq]
 
 lemma xor_eq_propagate (x y : ℕ → Bool) :
-  xor_seq x y = propagate empty.elim
-    (λ _ (y : Bool → Bool), (empty.elim, bxor (y tt) (y ff))) (λ b, cond b x y) :=
-by ext n; cases n; simp [propagate, propagateAux, xor_seq]
+    xorSeq x y = propagate Empty.elim
+      (λ _ (y : Bool → Bool) => (Empty.elim, xor (y true) (y false))) (λ b => cond b x y) := by
+  ext n; cases n <;> simp [propagate, propagateAux, xorSeq]
 
 lemma not_eq_propagate (x : ℕ → Bool) :
-  not_seq x = propagate empty.elim (λ _ (y : unit → Bool), (empty.elim, bnot (y ()))) (λ _, x) :=
-by ext n; cases n; simp [propagate, propagateAux, not_seq]
+    notSeq x = propagate Empty.elim (λ _ (y : Unit → Bool) => (Empty.elim, !(y ()))) (λ _ => x) := by
+  ext n; cases n <;> simp [propagate, propagateAux, notSeq]
 
 lemma ls_eq_propagate (x : ℕ → Bool) :
-  ls_seq x = propagate (λ _ : unit, ff) (λ (carry x : unit → Bool), (x, carry ())) (λ _, x) :=
+  lsSeq x = propagate (λ _ : Unit => false) (λ (carry x : Unit → Bool) => (x, carry ())) (λ _ => x) :=
 begin
   ext n,
   cases n with n,
   { refl },
   { cases n,
-    { simp [ls_seq, propagate_succ] },
-    { simp [ls_seq, propagate_succ] } }
+    { simp [lsSeq, propagate_succ] },
+    { simp [lsSeq, propagate_succ] } }
 end
 
-lemma add_seqAux_eq_propagate_carry (x y : ℕ → Bool) (n : ℕ) :
-  (add_seqAux x y n).2 = propagate_carry (λ _, ff)
-    (λ (carry : unit → Bool) (bits : Bool → Bool),
-      λ _, (bits tt && bits ff) || (bits ff && carry ()) || (bits tt && carry ()))
+lemma add_seqAux_eq_propagateCarry (x y : ℕ → Bool) (n : ℕ) :
+  (add_seqAux x y n).2 = propagateCarry (λ _, false)
+    (λ (carry : Unit → Bool) (bits : Bool → Bool),
+      λ _, (bits true && bits false) || (bits false && carry ()) || (bits true && carry ()))
   (λ b, cond b x y) n () :=
 begin
   induction n,
@@ -298,10 +291,10 @@ begin
 end
 
 lemma add_eq_propagate (x y : ℕ → Bool) :
-  add_seq x y = propagate (λ _, ff)
-    (λ (carry : unit → Bool) (bits : Bool → Bool),
-      (λ _, (bits tt && bits ff) || (bits ff && carry ()) || (bits tt && carry ()),
-        bxor (bits tt) (bxor (bits ff) (carry ()))))
+  add_seq x y = propagate (λ _, false)
+    (λ (carry : Unit → Bool) (bits : Bool → Bool),
+      (λ _, (bits true && bits false) || (bits false && carry ()) || (bits true && carry ()),
+        bxor (bits true) (bxor (bits false) (carry ()))))
   (λ b, cond b x y) :=
 begin
   ext n,
@@ -309,15 +302,15 @@ begin
   { simp [add_seq, add_seqAux] },
   { cases n,
     { simp [add_seq, add_seqAux, propagate_succ] },
-    { simp [add_seq, add_seqAux, add_seqAux_eq_propagate_carry,
+    { simp [add_seq, add_seqAux, add_seqAux_eq_propagateCarry,
         propagate_succ] } }
 end
 
-lemma sub_seqAux_eq_propagate_carry (x y : ℕ → Bool) (n : ℕ) :
-  (sub_seqAux x y n).2 = propagate_carry (λ _, ff)
-    (λ (carry : unit → Bool) (bits : Bool → Bool),
-      λ _, (bnot (bits tt) && (bits ff)) ||
-        (bnot (bxor (bits tt) (bits ff))) && carry ())
+lemma sub_seqAux_eq_propagateCarry (x y : ℕ → Bool) (n : ℕ) :
+  (sub_seqAux x y n).2 = propagateCarry (λ _, false)
+    (λ (carry : Unit → Bool) (bits : Bool → Bool),
+      λ _, (bnot (bits true) && (bits false)) ||
+        (bnot (bxor (bits true) (bits false))) && carry ())
   (λ b, cond b x y) n () :=
 begin
   induction n,
@@ -326,11 +319,11 @@ begin
 end
 
 lemma sub_eq_propagate (x y : ℕ → Bool) :
-  sub_seq x y = propagate (λ _, ff)
-    (λ (carry : unit → Bool) (bits : Bool → Bool),
-      (λ _, (bnot (bits tt) && (bits ff)) ||
-        ((bnot (bxor (bits tt) (bits ff))) && carry ()),
-        bxor (bits tt) (bxor (bits ff) (carry ()))))
+  sub_seq x y = propagate (λ _, false)
+    (λ (carry : Unit → Bool) (bits : Bool → Bool),
+      (λ _, (bnot (bits true) && (bits false)) ||
+        ((bnot (bxor (bits true) (bits false))) && carry ()),
+        bxor (bits true) (bxor (bits false) (carry ()))))
   (λ b, cond b x y) :=
 begin
   ext n,
@@ -338,96 +331,96 @@ begin
   { simp [sub_seq, sub_seqAux] },
   { cases n,
     { simp [sub_seq, sub_seqAux, propagate_succ] },
-    { simp [sub_seq, sub_seqAux, sub_seqAux_eq_propagate_carry,
+    { simp [sub_seq, sub_seqAux, sub_seqAux_eq_propagateCarry,
         propagate_succ] } }
 end
 
-lemma neg_seqAux_eq_propagate_carry (x : ℕ → Bool) (n : ℕ) :
-  (neg_seqAux x n).2 = propagate_carry (λ _, tt)
-    (λ (carry : unit → Bool) (bits : unit → Bool),
+lemma negSeqAux_eq_propagateCarry (x : ℕ → Bool) (n : ℕ) :
+  (negSeqAux x n).2 = propagateCarry (λ _, true)
+    (λ (carry : Unit → Bool) (bits : Unit → Bool),
       λ _, (bnot (bits ())) && (carry ()))
   (λ _, x) n () :=
 begin
   induction n,
-  { simp [neg_seqAux] },
-  { simp [neg_seqAux, *] }
+  { simp [negSeqAux] },
+  { simp [negSeqAux, *] }
 end
 
 lemma neg_eq_propagate (x : ℕ → Bool) :
-  neg_seq x = propagate (λ _, tt)
-    (λ (carry : unit → Bool) (bits : unit → Bool),
+  negSeq x = propagate (λ _, true)
+    (λ (carry : Unit → Bool) (bits : Unit → Bool),
       (λ _, (bnot (bits ())) && (carry ()), bxor (bnot (bits ())) (carry ())))
   (λ _, x) :=
 begin
   ext n,
   cases n with n,
-  { simp [neg_seq, neg_seqAux] },
+  { simp [negSeq, negSeqAux] },
   { cases n,
-    { simp [neg_seq, neg_seqAux, propagate_succ] },
-    { simp [neg_seq, neg_seqAux, neg_seqAux_eq_propagate_carry,
+    { simp [negSeq, negSeqAux, propagate_succ] },
+    { simp [negSeq, negSeqAux, negSeqAux_eq_propagateCarry,
         propagate_succ] } }
 end
 
-lemma incr_seqAux_eq_propagate_carry (x : ℕ → Bool) (n : ℕ) :
-  (incr_seqAux x n).2 = propagate_carry (λ _, tt)
-    (λ (carry : unit → Bool) (bits : unit → Bool),
+lemma incrSeqAux_eq_propagateCarry (x : ℕ → Bool) (n : ℕ) :
+  (incrSeqAux x n).2 = propagateCarry (λ _, true)
+    (λ (carry : Unit → Bool) (bits : Unit → Bool),
       λ _, (bits ()) && carry ())
   (λ _, x) n () :=
 begin
   induction n,
-  { simp [incr_seqAux] },
-  { simp [incr_seqAux, *] }
+  { simp [incrSeqAux] },
+  { simp [incrSeqAux, *] }
 end
 
 lemma incr_eq_propagate (x : ℕ → Bool) :
-  incr_seq x = propagate (λ _, tt)
-    (λ (carry : unit → Bool) (bits : unit → Bool),
+  incrSeq x = propagate (λ _, true)
+    (λ (carry : Unit → Bool) (bits : Unit → Bool),
       (λ _, (bits ()) && carry (), bxor (bits ()) (carry ())))
   (λ _, x) :=
 begin
   ext n,
   cases n with n,
-  { simp [incr_seq, incr_seqAux] },
+  { simp [incrSeq, incrSeqAux] },
   { cases n,
-    { simp [incr_seq, incr_seqAux, propagate_succ] },
-    { simp [incr_seq, incr_seqAux, incr_seqAux_eq_propagate_carry,
+    { simp [incrSeq, incrSeqAux, propagate_succ] },
+    { simp [incrSeq, incrSeqAux, incrSeqAux_eq_propagateCarry,
         propagate_succ] } }
 end
 
-lemma decr_seqAux_eq_propagate_carry (x : ℕ → Bool) (n : ℕ) :
-  (decr_seqAux x n).2 = propagate_carry (λ _, tt)
-    (λ (carry : unit → Bool) (bits : unit → Bool),
+lemma decrSeqAux_eq_propagateCarry (x : ℕ → Bool) (n : ℕ) :
+  (decrSeqAux x n).2 = propagateCarry (λ _, true)
+    (λ (carry : Unit → Bool) (bits : Unit → Bool),
       λ _, (bnot (bits ())) && carry ())
   (λ _, x) n () :=
 begin
   induction n,
-  { simp [decr_seqAux] },
-  { simp [decr_seqAux, *] }
+  { simp [decrSeqAux] },
+  { simp [decrSeqAux, *] }
 end
 
 lemma decr_eq_propagate (x : ℕ → Bool) :
-  decr_seq x = propagate (λ _, tt)
-    (λ (carry : unit → Bool) (bits : unit → Bool),
+  decrSeq x = propagate (λ _, true)
+    (λ (carry : Unit → Bool) (bits : Unit → Bool),
       (λ _, (bnot (bits ())) && carry (), bxor (bits ()) (carry ())))
   (λ _, x) :=
 begin
   ext n,
   cases n with n,
-  { simp [decr_seq, decr_seqAux] },
+  { simp [decrSeq, decrSeqAux] },
   { cases n,
-    { simp [decr_seq, decr_seqAux, propagate_succ] },
-    { simp [decr_seq, decr_seqAux, decr_seqAux_eq_propagate_carry,
+    { simp [decrSeq, decrSeqAux, propagate_succ] },
+    { simp [decrSeq, decrSeqAux, decrSeqAux_eq_propagateCarry,
         propagate_succ] } }
 end
 
 structure propagate_struc (arity : Type) : Type 1 :=
 ( α  : Type )
-[ i : fintype α ]
+[ i : Fintype α ]
 ( init_carry : α → Bool )
 ( next_bit : ∀ (carry : α → Bool) (bits : arity → Bool),
     (α → Bool) × Bool )
 
-attribute [instance] propagate_struc.i
+atrueribute [instance] propagate_struc.i
 
 namespace propagate_struc
 
@@ -436,12 +429,12 @@ variables {arity : Type} (p : propagate_struc arity)
 def eval : (arity → ℕ → Bool) → ℕ → Bool :=
 propagate p.init_carry p.next_bit
 
-def change_vars {arity2 : Type} (change_vars : arity → arity2) :
+def changeVars {arity2 : Type} (changeVars : arity → arity2) :
   propagate_struc arity2 :=
 { α := p.α,
   i := p.i,
   init_carry := p.init_carry,
-  next_bit := λ carry bits, p.next_bit carry (λ i, bits (change_vars i)) }
+  next_bit := λ carry bits, p.next_bit carry (fun i => bits (changeVars i)) }
 
 def compose [fintype arity]
   (new_arity : Type)
@@ -451,12 +444,12 @@ def compose [fintype arity]
   propagate_struc (new_arity) :=
 { α := p.α ⊕ (Σ a, (q a).α),
   i := by letI := p.i; apply_instance,
-  init_carry := sum.elim p.init_carry (λ x, (q x.1).init_carry x.2),
+  init_carry := Sum.elim p.init_carry (λ x, (q x.1).init_carry x.2),
   next_bit := λ carry bits,
     let f : ∀ (a : arity), ((q a).α → Bool) × Bool := λ a, (q a).next_bit (λ d,
         carry (inr ⟨a, d⟩)) (λ d, bits (vars a d)) in
     let g : (p.α → Bool) × Bool := (p.next_bit (carry ∘ inl) (λ a, (f a).2)) in
-    (sum.elim g.1 (λ x, (f x.1).1 x.2), g.2) }
+    (Sum.elim g.1 (λ x, (f x.1).1 x.2), g.2) }
 
 lemma eval_compose [fintype arity]
   (new_arity : Type)
@@ -465,7 +458,7 @@ lemma eval_compose [fintype arity]
   (q : ∀ (a : arity), propagate_struc (q_arity a))
   (x : new_arity → ℕ → Bool):
   (p.compose new_arity q_arity vars q).eval x =
-  p.eval (λ a, (q a).eval (λ i, x (vars _ i))) :=
+  p.eval (λ a, (q a).eval (fun i => x (vars _ i))) :=
 begin
   ext n,
   simp only [eval, compose, propagate_propagate]
@@ -474,39 +467,39 @@ end
 def and : propagate_struc Bool :=
 { α := empty,
   i := by apply_instance,
-  init_carry := empty.elim,
-  next_bit := λ carry bits, (empty.elim, bits tt && bits ff) }
+  init_carry := Empty.elim,
+  next_bit := λ carry bits, (Empty.elim, bits true && bits false) }
 
-@[simp] lemma eval_and (x : Bool → ℕ → Bool) : and.eval x = and_seq (x tt) (x ff) :=
-by ext n; cases n; simp [and, and_seq, eval, propagate_succ]
+@[simp] lemma eval_and (x : Bool → ℕ → Bool) : and.eval x = andSeq (x true) (x false) :=
+by ext n; cases n; simp [and, andSeq, eval, propagate_succ]
 
 def or : propagate_struc Bool :=
 { α := empty,
   i := by apply_instance,
-  init_carry := empty.elim,
-  next_bit := λ carry bits, (empty.elim, bits tt || bits ff) }
+  init_carry := Empty.elim,
+  next_bit := λ carry bits, (Empty.elim, bits true || bits false) }
 
-@[simp] lemma eval_or (x : Bool → ℕ → Bool) : or.eval x = or_seq (x tt) (x ff) :=
-by ext n; cases n; simp [or, or_seq, eval, propagate_succ]
+@[simp] lemma eval_or (x : Bool → ℕ → Bool) : or.eval x = orSeq (x true) (x false) :=
+by ext n; cases n; simp [or, orSeq, eval, propagate_succ]
 
 def xor : propagate_struc Bool :=
 { α := empty,
   i := by apply_instance,
-  init_carry := empty.elim,
-  next_bit := λ carry bits, (empty.elim, bxor (bits tt) (bits ff)) }
+  init_carry := Empty.elim,
+  next_bit := λ carry bits, (Empty.elim, bxor (bits true) (bits false)) }
 
-@[simp] lemma eval_xor (x : Bool → ℕ → Bool) : xor.eval x = xor_seq (x tt) (x ff) :=
-by ext n; cases n; simp [xor, xor_seq, eval, propagate_succ]
+@[simp] lemma eval_xor (x : Bool → ℕ → Bool) : xor.eval x = xorSeq (x true) (x false) :=
+by ext n; cases n; simp [xor, xorSeq, eval, propagate_succ]
 
 def add : propagate_struc Bool :=
-{ α := unit,
+{ α := Unit,
   i := by apply_instance,
-  init_carry := λ _, ff,
-  next_bit := λ (carry : unit → Bool) (bits : Bool → Bool),
-      (λ _, (bits tt && bits ff) || (bits ff && carry ()) || (bits tt && carry ()),
-        bxor (bits tt) (bxor (bits ff) (carry ()))) }
+  init_carry := λ _, false,
+  next_bit := λ (carry : Unit → Bool) (bits : Bool → Bool),
+      (λ _, (bits true && bits false) || (bits false && carry ()) || (bits true && carry ()),
+        bxor (bits true) (bxor (bits false) (carry ()))) }
 
-@[simp] lemma eval_add (x : Bool → ℕ → Bool) : add.eval x = add_seq (x tt) (x ff) :=
+@[simp] lemma eval_add (x : Bool → ℕ → Bool) : add.eval x = add_seq (x true) (x false) :=
 begin
   dsimp [add, eval],
   rw [add_eq_propagate],
@@ -516,15 +509,15 @@ begin
 end
 
 def sub : propagate_struc Bool :=
-{ α := unit,
+{ α := Unit,
   i := by apply_instance,
-  init_carry := λ _, ff,
-  next_bit := λ (carry : unit → Bool) (bits : Bool → Bool),
-      (λ _, (bnot (bits tt) && (bits ff)) ||
-        ((bnot (bxor (bits tt) (bits ff))) && carry ()),
-        bxor (bits tt) (bxor (bits ff) (carry ()))) }
+  init_carry := λ _, false,
+  next_bit := λ (carry : Unit → Bool) (bits : Bool → Bool),
+      (λ _, (bnot (bits true) && (bits false)) ||
+        ((bnot (bxor (bits true) (bits false))) && carry ()),
+        bxor (bits true) (bxor (bits false) (carry ()))) }
 
-@[simp] lemma eval_sub (x : Bool → ℕ → Bool) : sub.eval x = sub_seq (x tt) (x ff) :=
+@[simp] lemma eval_sub (x : Bool → ℕ → Bool) : sub.eval x = sub_seq (x true) (x false) :=
 begin
   dsimp [sub, eval],
   rw [sub_eq_propagate],
@@ -533,14 +526,14 @@ begin
   cases b; refl
 end
 
-def neg : propagate_struc unit :=
-{ α := unit,
+def neg : propagate_struc Unit :=
+{ α := Unit,
   i := by apply_instance,
-  init_carry := λ _, tt,
-  next_bit := λ (carry : unit → Bool) (bits : unit → Bool),
+  init_carry := λ _, true,
+  next_bit := λ (carry : Unit → Bool) (bits : Unit → Bool),
     (λ _, (bnot (bits ())) && (carry ()), bxor (bnot (bits ())) (carry ())) }
 
-@[simp] lemma eval_neg (x : unit → ℕ → Bool) : neg.eval x = neg_seq (x ()) :=
+@[simp] lemma eval_neg (x : Unit → ℕ → Bool) : neg.eval x = negSeq (x ()) :=
 begin
   dsimp [neg, eval],
   rw [neg_eq_propagate],
@@ -549,67 +542,67 @@ begin
   cases b; refl
 end
 
-def not : propagate_struc unit :=
+def not : propagate_struc Unit :=
 { α := empty,
   i := by apply_instance,
-  init_carry := empty.elim,
-  next_bit := λ carry bits, (empty.elim, bnot (bits ())) }
+  init_carry := Empty.elim,
+  next_bit := λ carry bits, (Empty.elim, bnot (bits ())) }
 
-@[simp] lemma eval_not (x : unit → ℕ → Bool) : not.eval x = not_seq (x ()) :=
-by ext n; cases n; simp [not, not_seq, eval, propagate_succ]
+@[simp] lemma eval_not (x : Unit → ℕ → Bool) : not.eval x = notSeq (x ()) :=
+by ext n; cases n; simp [not, notSeq, eval, propagate_succ]
 
 def zero : propagate_struc (fin 0) :=
 { α := empty,
   i := by apply_instance,
-  init_carry := empty.elim,
-  next_bit := λ carry bits, (empty.elim, ff) }
+  init_carry := Empty.elim,
+  next_bit := λ carry bits, (Empty.elim, false) }
 
-@[simp] lemma eval_zero (x : fin 0 → ℕ → Bool) : zero.eval x = zero_seq :=
-by ext n; cases n; simp [zero, zero_seq, eval, propagate_succ]
+@[simp] lemma eval_zero (x : Fin 0 → ℕ → Bool) : zero.eval x = zeroSeq :=
+by ext n; cases n; simp [zero, zeroSeq, eval, propagate_succ]
 
 def one : propagate_struc (fin 0) :=
-{ α := unit,
+{ α := Unit,
   i := by apply_instance,
-  init_carry := λ _, tt,
-  next_bit := λ carry bits, (λ _, ff, carry ()) }
+  init_carry := λ _, true,
+  next_bit := λ carry bits, (λ _, false, carry ()) }
 
-@[simp] lemma eval_one (x : fin 0 → ℕ → Bool) : one.eval x = one_seq :=
-by ext n; cases n; simp [one, one_seq, eval, propagate_succ2]
+@[simp] lemma eval_one (x : Fin 0 → ℕ → Bool) : one.eval x = oneSeq :=
+by ext n; cases n; simp [one, oneSeq, eval, propagate_succ2]
 
 def neg_one : propagate_struc (fin 0) :=
 { α := empty,
   i := by apply_instance,
-  init_carry := empty.elim,
-  next_bit := λ carry bits, (empty.elim, tt) }
+  init_carry := Empty.elim,
+  next_bit := λ carry bits, (Empty.elim, true) }
 
-@[simp] lemma eval_neg_one (x : fin 0 → ℕ → Bool) : neg_one.eval x = neg_one_seq :=
-by ext n; cases n; simp [neg_one, neg_one_seq, eval, propagate_succ2]
+@[simp] lemma eval_neg_one (x : Fin 0 → ℕ → Bool) : neg_one.eval x = neg_oneSeq :=
+by ext n; cases n; simp [neg_one, neg_oneSeq, eval, propagate_succ2]
 
-def ls : propagate_struc unit :=
-{ α := unit,
+def ls : propagate_struc Unit :=
+{ α := Unit,
   i := by apply_instance,
-  init_carry := λ _, ff,
+  init_carry := λ _, false,
   next_bit := λ carry bits, (bits, carry ()) }
 
-@[simp] lemma eval_ls (x : unit → ℕ → Bool) : ls.eval x = ls_seq (x ()) :=
-by ext n; cases n; simp [ls, ls_seq, eval, propagate_succ2]
+@[simp] lemma eval_ls (x : Unit → ℕ → Bool) : ls.eval x = lsSeq (x ()) :=
+by ext n; cases n; simp [ls, lsSeq, eval, propagate_succ2]
 
 def var (n : ℕ) : propagate_struc (fin (n+1)) :=
 { α := empty,
   i := by apply_instance,
-  init_carry := empty.elim,
-  next_bit := λ carry bits, (empty.elim, bits (fin.last n)) }
+  init_carry := Empty.elim,
+  next_bit := λ carry bits, (Empty.elim, bits (Fin.last n)) }
 
-@[simp] lemma eval_var (n : ℕ) (x : fin (n+1) → ℕ → Bool) : (var n).eval x = x (fin.last n) :=
+@[simp] lemma eval_var (n : ℕ) (x : Fin (n+1) → ℕ → Bool) : (var n).eval x = x (Fin.last n) :=
 by ext m; cases m; simp [var, eval, propagate_succ]
 
-def incr : propagate_struc unit :=
-{ α := unit,
+def incr : propagate_struc Unit :=
+{ α := Unit,
   i := by apply_instance,
-  init_carry := λ _, tt,
+  init_carry := λ _, true,
   next_bit := λ carry bits, (λ _, bits () && carry (), bxor (bits ()) (carry ())) }
 
-@[simp] lemma eval_incr (x : unit → ℕ → Bool) : incr.eval x = incr_seq (x ()) :=
+@[simp] lemma eval_incr (x : Unit → ℕ → Bool) : incr.eval x = incrSeq (x ()) :=
 begin
   dsimp [incr, eval],
   rw [incr_eq_propagate],
@@ -618,13 +611,13 @@ begin
   cases b; refl
 end
 
-def decr : propagate_struc unit :=
-{ α := unit,
+def decr : propagate_struc Unit :=
+{ α := Unit,
   i := by apply_instance,
-  init_carry := λ _, tt,
+  init_carry := λ _, true,
   next_bit := λ carry bits, (λ _, bnot (bits ()) && carry (), bxor (bits ()) (carry ())) }
 
-@[simp] lemma eval_decr (x : unit → ℕ → Bool) : decr.eval x = decr_seq (x ()) :=
+@[simp] lemma eval_decr (x : Unit → ℕ → Bool) : decr.eval x = decrSeq (x ()) :=
 begin
   dsimp [decr, eval],
   rw [decr_eq_propagate],
@@ -635,12 +628,12 @@ end
 
 end propagate_struc
 
-structure propagate_solution (t : term) extends propagate_struc (fin (arity t)) :=
-( good : t.eval_fin = to_propagate_struc.eval )
+structure propagate_solution (t : Term) extends propagate_struc (fin (arity t)) :=
+( good : t.evalFin = to_propagate_struc.eval )
 
 def compose_unary
-  (p : propagate_struc unit)
-  {t : term}
+  (p : propagate_struc Unit)
+  {t : Term}
   (q : propagate_solution t) :
   propagate_struc (fin (arity t)) :=
 p.compose
@@ -651,21 +644,21 @@ p.compose
 
 def compose_binary
   (p : propagate_struc Bool)
-  {t₁ t₂ : term}
+  {t₁ t₂ : Term}
   (q₁ : propagate_solution t₁)
   (q₂ : propagate_solution t₂) :
   propagate_struc (fin (max (arity t₁) (arity t₂))) :=
 p.compose (fin (max (arity t₁) (arity t₂)))
   (λ b, fin (cond b (arity t₁) (arity t₂)))
-  (λ b i, fin.cast_le (by cases b; simp) i)
+  (λ b i, Fin.castLe (by cases b; simp) i)
   (λ b, Bool.rec q₂.to_propagate_struc q₁.to_propagate_struc b)
 
 @[simp] lemma compose_unary_eval
-  (p : propagate_struc unit)
-  {t : term}
+  (p : propagate_struc Unit)
+  {t : Term}
   (q : propagate_solution t)
-  (x : fin (arity t) → ℕ → Bool) :
-  (compose_unary p q).eval x = p.eval (λ _, t.eval_fin x) :=
+  (x : Fin (arity t) → ℕ → Bool) :
+  (compose_unary p q).eval x = p.eval (λ _, t.evalFin x) :=
 begin
   rw [compose_unary, propagate_struc.eval_compose, q.good],
   refl
@@ -673,13 +666,13 @@ end
 
 @[simp] lemma compose_binary_eval
   (p : propagate_struc Bool)
-  {t₁ t₂ : term}
+  {t₁ t₂ : Term}
   (q₁ : propagate_solution t₁)
   (q₂ : propagate_solution t₂)
-  (x : fin (max (arity t₁) (arity t₂)) → ℕ → Bool) :
+  (x : Fin (max (arity t₁) (arity t₂)) → ℕ → Bool) :
   (compose_binary p q₁ q₂).eval x = p.eval
-    (λ b, cond b (t₁.eval_fin (λ i, x (fin.cast_le (by simp) i)))
-                 (t₂.eval_fin (λ i, x (fin.cast_le (by simp) i)))) :=
+    (λ b, cond b (t₁.evalFin (fun i => x (Fin.castLe (by simp) i)))
+                 (t₂.evalFin (fun i => x (Fin.castLe (by simp) i)))) :=
 begin
   rw [compose_binary, propagate_struc.eval_compose, q₁.good, q₂.good],
   congr,
@@ -709,20 +702,20 @@ lemma cond_propagate {α α' β β' : Type}
     (show cond b β β' → ℕ → Bool, from Bool.rec (λ b, (x (fβ' b))) (λ b, (x (fβ b))) b) :=
 by cases b; refl
 
-def term_eval_eq_propagate : ∀ (t : term),
+def term_eval_eq_propagate : ∀ (t : Term),
   propagate_solution t
 | (var n) :=
   { to_propagate_struc := propagate_struc.var n,
-    good := by ext; simp [term.eval_fin] }
+    good := by ext; simp [Term.evalFin] }
 | zero :=
   { to_propagate_struc := propagate_struc.zero,
-    good := by ext; simp [term.eval_fin] }
+    good := by ext; simp [Term.evalFin] }
 | one :=
   { to_propagate_struc := propagate_struc.one,
-    good := by ext; simp [term.eval_fin] }
+    good := by ext; simp [Term.evalFin] }
 | neg_one :=
   { to_propagate_struc := propagate_struc.neg_one,
-    good := by ext; simp [term.eval_fin] }
+    good := by ext; simp [Term.evalFin] }
 | (and t₁ t₂) :=
   let q₁ := term_eval_eq_propagate t₁ in
   let q₂ := term_eval_eq_propagate t₂ in
@@ -779,9 +772,9 @@ variables [fintype α] [fintype α']
 open fintype
 
 lemma exists_repeat_carry (seq : β → ℕ → Bool) :
-  ∃ n m : fin (2 ^ (card α) + 1),
-    propagate_carry2 init_carry next_carry seq n =
-    propagate_carry2 init_carry next_carry seq m ∧
+  ∃ n m : Fin (2 ^ (card α) + 1),
+    propagateCarry2 init_carry next_carry seq n =
+    propagateCarry2 init_carry next_carry seq m ∧
     n < m :=
 begin
   by_contra h,
@@ -791,16 +784,16 @@ begin
   simpa using fintype.card_le_of_injective _ this
 end
 
-lemma propagate_carry2_eq_of_seq_eq_lt (seq₁ seq₂ : β → ℕ → Bool)
+lemma propagateCarry2_eq_of_seq_eq_lt (seq₁ seq₂ : β → ℕ → Bool)
   (init_carry : α → Bool)
   (next_carry : ∀ (carry : α → Bool) (bits : β → Bool), (α → Bool))
   (i : ℕ) (h : ∀ (b) j < i, seq₁ b j = seq₂ b j) :
-  propagate_carry2 init_carry next_carry seq₁ i =
-    propagate_carry2 init_carry next_carry seq₂ i :=
+  propagateCarry2 init_carry next_carry seq₁ i =
+    propagateCarry2 init_carry next_carry seq₂ i :=
 begin
   induction i with i ih,
-  { simp [propagate_carry2] },
-  { simp [propagate_carry2, h _ i (nat.lt_succ_self i)],
+  { simp [propagateCarry2] },
+  { simp [propagateCarry2, h _ i (nat.lt_succ_self i)],
     rw ih,
     exact λ b j hj, h b j (nat.lt_succ_of_lt hj) }
 end
@@ -816,26 +809,26 @@ begin
   { simp [propagate_zero, h _ 0 (le_refl _)] },
   { simp only [propagate_succ2, propagate_succ2, h _ _ (le_refl _)],
     congr' 2,
-    apply propagate_carry2_eq_of_seq_eq_lt,
+    apply propagateCarry2_eq_of_seq_eq_lt,
     exact λ b j hj, h b j (le_of_lt hj) }
 end
 
-lemma propagate_carry2_eq_of_carry_eq (seq₁ seq₂ : β → ℕ → Bool)
+lemma propagateCarry2_eq_of_carry_eq (seq₁ seq₂ : β → ℕ → Bool)
   (m n : ℕ)
-  (h₁ : propagate_carry2 init_carry
+  (h₁ : propagateCarry2 init_carry
     (λ carry bits, (next_bit carry bits).1) seq₁ m =
-       propagate_carry2 init_carry
+       propagateCarry2 init_carry
     (λ carry bits, (next_bit carry bits).1) seq₂ n) (x : ℕ)
   (h₃ : ∀ y b, y ≤ x → seq₁ b (m + y) = seq₂ b (n + y))  :
-  propagate_carry2 init_carry
+  propagateCarry2 init_carry
     (λ carry bits, (next_bit carry bits).1) seq₁ (m + x) =
-  propagate_carry2 init_carry
+  propagateCarry2 init_carry
     (λ carry bits, (next_bit carry bits).1) seq₂ (n + x) :=
 begin
   induction x with x ih generalizing seq₁ seq₂,
   { simp * at * },
   { simp only [h₃ x _ (nat.le_succ _),
-      nat.add_succ, propagate_carry2, add_zero] at *,
+      nat.add_succ, propagateCarry2, add_zero] at *,
     rw [ih],
     assumption,
     exact λ y b h, h₃ y b (nat.le_succ_of_le h) }
@@ -843,9 +836,9 @@ end
 
 lemma propagate_eq_of_carry_eq (seq₁ seq₂ : β → ℕ → Bool)
   (m n : ℕ)
-  (h₁ : propagate_carry2 init_carry
+  (h₁ : propagateCarry2 init_carry
     (λ carry bits, (next_bit carry bits).1) seq₁ m =
-       propagate_carry2 init_carry
+       propagateCarry2 init_carry
     (λ carry bits, (next_bit carry bits).1) seq₂ n) (x : ℕ)
   (h₃ : ∀ y b, y ≤ x → seq₁ b (m + y) = seq₂ b (n + y))  :
   propagate init_carry next_bit seq₁ (m + x) =
@@ -854,7 +847,7 @@ begin
   cases x,
   { cases m,
     { cases n,
-      { simp [h₃ 0 _ (le_refl _), propagate_carry2, *] at * },
+      { simp [h₃ 0 _ (le_refl _), propagateCarry2, *] at * },
       { simp [*, h₃ 0 _ (le_refl _), propagate_succ2] at *,
         rw [← h₁] } },
     { cases n,
@@ -866,26 +859,26 @@ begin
   { simp only [nat.add_succ, propagate_succ2, add_zero],
     simp [← nat.add_succ, h₃ _ _ (le_refl _)],
     congr' 2,
-    apply propagate_carry2_eq_of_carry_eq,
+    apply propagateCarry2_eq_of_carry_eq,
     assumption,
     assumption }
 end
 
-lemma propagate_carry_propagate_carry_add (x : β → ℕ → Bool) :
+lemma propagateCarry_propagateCarry_add (x : β → ℕ → Bool) :
   ∀ (init_carry : α → Bool)
     (next_carry : ∀ (carry : α → Bool) (bits : β → Bool), (α → Bool)),
   ∀ n i : ℕ,
-  propagate_carry2 (propagate_carry2 init_carry next_carry x n)
+  propagateCarry2 (propagateCarry2 init_carry next_carry x n)
     next_carry (λ b k, x b (k + n)) i =
-  propagate_carry2 init_carry next_carry x (i + n)
-| init_carry next_carry 0 0 := by simp [propagate_carry2]
+  propagateCarry2 init_carry next_carry x (i + n)
+| init_carry next_carry 0 0 := by simp [propagateCarry2]
 | init_carry next_carry (n+1) 0 :=
-  by simp [propagate_carry, propagate_carry2_succ]
+  by simp [propagateCarry, propagateCarry2_succ]
 | init_carry next_carry n (i+1) := begin
-  rw [propagate_carry2, add_assoc,
-    propagate_carry_propagate_carry_add],
+  rw [propagateCarry2, add_assoc,
+    propagateCarry_propagateCarry_add],
   simp only [nat.one_add, nat.add_one, nat.succ_add, nat.add_succ,
-    add_zero, propagate_carry2, zero_add]
+    add_zero, propagateCarry2, zero_add]
 end
 
 lemma exists_repeat : ∀ (seq : β → ℕ → Bool)
@@ -896,11 +889,11 @@ lemma exists_repeat : ∀ (seq : β → ℕ → Bool)
 begin
   by_cases hn2 : n < 2 ^ card α,
   { exact ⟨n, hn2, seq, rfl⟩ },
-  { rcases exists_repeat_carry (propagate_carry2 init_carry (λ c b, (next_bit c b).1) seq
+  { rcases exists_repeat_carry (propagateCarry2 init_carry (λ c b, (next_bit c b).1) seq
         (n - 2 ^ card α))
       (λ carry bits, (next_bit  carry bits).1)
       (λ b i, seq b (i + (n - 2^ (card α)))) with ⟨a, b, h₁, h₂⟩,
-    simp only [propagate_carry_propagate_carry_add] at h₁,
+    simp only [propagateCarry_propagateCarry_add] at h₁,
     rcases have wf : n - (b - a) < n,
         from nat.sub_lt (lt_of_lt_of_le (pow_pos two_pos _) (le_of_not_gt hn2))
           (nat.sub_pos_of_lt h₂),
@@ -933,10 +926,10 @@ begin
         exact le_of_lt h₂,
         simp * at * },
       rw [← h₁],
-      apply propagate_carry2_eq_of_seq_eq_lt,
-      simp { contextual := tt } },
+      apply propagateCarry2_eq_of_seq_eq_lt,
+      simp { contextual := true } },
     { intros y c hc,
-      simp only [add_lt_iff_neg_left, not_lt_zero', if_false],
+      simp only [add_lt_ifalse_neg_left, not_lt_zero', if_false],
       congr' 1,
       zify,
       rw [nat.cast_sub, nat.cast_sub],
@@ -946,24 +939,24 @@ begin
 end
 using_well_founded { rel_tac := λ _ _, `[exact ⟨_, measure_wf psigma.snd⟩] }
 
-lemma propagate_eq_zero_iff (init_carry : α → Bool)
+lemma propagate_eq_zero_ifalse (init_carry : α → Bool)
   (next_bit : ∀ (carry : α → Bool) (bits : β → Bool), (α → Bool) × Bool) :
-  (∀ seq, propagate init_carry next_bit seq = zero_seq) ↔
-  (∀ seq, ∀ i < 2 ^ (card α), propagate init_carry next_bit seq i = ff) :=
+  (∀ seq, propagate init_carry next_bit seq = zeroSeq) ↔
+  (∀ seq, ∀ i < 2 ^ (card α), propagate init_carry next_bit seq i = false) :=
 begin
   split,
   { intros h i _,
-    simp [h, zero_seq] },
+    simp [h, zeroSeq] },
   { intros h seq,
     funext i,
     rcases exists_repeat init_carry next_bit seq i with ⟨j, hj, seq2, hseq2⟩,
-    rw [← hseq2, h seq2 j hj, zero_seq] }
+    rw [← hseq2, h seq2 j hj, zeroSeq] }
 end
 
-lemma eq_iff_xor_seq_eq_zero (seq₁ seq₂ : ℕ → Bool) :
-  (∀ i, seq₁ i = seq₂ i) ↔ (∀ i, xor_seq seq₁ seq₂ i = zero_seq i) :=
+lemma eq_ifalse_xorSeq_eq_zero (seq₁ seq₂ : ℕ → Bool) :
+  (∀ i, seq₁ i = seq₂ i) ↔ (∀ i, xorSeq seq₁ seq₂ i = zeroSeq i) :=
 begin
-  simp [function.funext_iff, xor_seq, zero_seq],
+  simp [function.funext_ifalse, xorSeq, zeroSeq],
   split,
   { intros, simp * },
   { intros h a,
@@ -971,14 +964,14 @@ begin
     cases (seq₁ a); cases (seq₂ a); simp * at *, }
 end
 
-lemma eval_eq_iff_xor_seq_eq_zero (t₁ t₂ : term) :
-  t₁.eval = t₂.eval ↔ (t₁.xor t₂).eval_fin = λ _, zero_seq :=
+lemma eval_eq_ifalse_xorSeq_eq_zero (t₁ t₂ : Term) :
+  t₁.eval = t₂.eval ↔ (t₁.xor t₂).evalFin = λ _, zeroSeq :=
 begin
-  simp only [function.funext_iff, term.eval, term.eval_fin,
-    ← eq_iff_xor_seq_eq_zero, ← eval_fin_eq_eval],
+  simp only [function.funext_ifalse, Term.eval, Term.evalFin,
+    ← eq_ifalse_xorSeq_eq_zero, ← evalFin_eq_eval],
   split,
   { intros h seq n,
-    have := h (λ j, if hj : j < (arity (t₁.xor t₂)) then seq ⟨j, hj⟩ else λ _, ff) n,
+    have := h (λ j, if hj : j < (arity (t₁.xor t₂)) then seq ⟨j, hj⟩ else λ _, false) n,
     simp at this,
     convert this },
   { intros h seq m,
